Progress on elimination of refinement types

theories/refinement_elimination.v
@@ -8,32 +8,6 @@ From Ltac2 Require Import Printf.
 Import Constr.Unsafe.
 
 
-Set Default Proof Mode "Classic".
-
-
-
-(* Definition p (n : nat) : Prop := n >= 3. *)
-
-(* Definition t := { x : nat | p x }. *)
-
-(* Definition x : t := exist _ 3 (le_n 3). *)
-
-
-(* Definition identity {A : Type} : A -> A := fun x => x. *)
-
-(* Goal (proj1_sig x) >= 3. *)
-(*   step_one foo (exist p 3 (le_n 3)). *)
-(*   pose (y := exist p 3 (le_n 3)). *)
-(*   step_one foo2 y. *)
-(*   step_one bar (fun x : @sig nat p => exist p (proj1_sig x) (proj2_sig x)). *)
-(*   step_one baz (let z : @sig nat p := exist p 3 (le_n 3) in z). *)
-
-(*   step_one baz2 ((fun k : @sig nat p -> @sig nat p => k y) id). *)
-(*   (* This one does not work *) *)
-
-
-(*   step_one baz3 (fun k : @sig nat p -> @sig nat p => k y). *)
-(*   Abort. *)
 
 (* The trigger should be activated for any symbol that contains a refinement type in its type *)
 (* param p: symbol whose type contain a refinement type *)
@@ -88,24 +62,96 @@ Require Import refinement_elimination_elpi.
 Tactic Notation "step_one" ident(i) constr(x) :=
   elpi step_one_tac ltac_string:(i) ltac_term:(x).
 
+Tactic Notation "make_eq" constr(x) constr(y) :=
+  elpi make_eq ltac_term:(x) ltac_term:(y).
+
+(* Require Import Psatz. *)
+
+(* Eval compute in (fun n => Nat.add n 2). *)
+(* Eval lazy beta delta iota zeta in 10000%nat. *)
+
+(* Section Test. *)
+(*   Variable n m : nat. *)
+(*   Hypothesis H : n <= m. *)
+
+(*   Lemma foob : n <= m+1. lia. Defined. *)
+(*   Eval compute in foob. *)
+
+(*   Eval compute in @exist _ (fun n' => n' <= m + 1) n foob. *)
+
+(* End Test. *)
+
+(* Definition a := 2. *)
+
+(* Definition f : nat -> nat := fun _ => a. *)
+
+(* Goal False. *)
+(*   let f := eval hnf in f in *)
+(*   replace bar f. *)
+(*   Abort. *)
+
+Definition P : nat -> Prop := fun x => x >= 3.
+
+Definition tt := {x : nat | P x}.
+
+Definition v : tt := exist P 3 (le_n 3).
+
+Definition f : nat -> nat -> tt := fun _ _ => v.
+
+Definition g : tt -> tt := fun r => r.
+
+(* Fixpoint rep_sig (i : nat) : Set := *)
+(*   match i with *)
+(*     | 0 => nat *)
+(*     | S i' => @sig (rep_sig i') (fun x => x = x) *)
+(*   end. *)
+
+(* Eval hnf in (match (rep_sig 2) with _ => 4 end). *)
+
+(* Variable y : rep_sig 2. *)
+
+(* Eval hnf in (fix x () : Set := rep_sig 2 in x). *)
+
+(* Eval hnf in (fix rep_sig (i : (id nat)) : id Set := *)
+(*      match i with *)
+(*      | 0 => nat *)
+(*      | S i' => {x : rep_sig i' | x = x} *)
+(*      end). *)
+
+
+(* Section foo. *)
+(* Variable (A : Type) (x : A) (P : A -> Prop) (f : P x) (a : A) (e : x = a). *)
+(* Print eq_ind. *)
+
+
+
+(* Goal proj1_sig v - 1 >= 2. *)
+(*   let f1 := fresh "step_one" in *)
+(*   step_one f1 (match id e in (_ = a0) return (id (P a0)) with | eq_refl => f end). *)
+
+(*   step_one foo v. *)
+(*   step_one bar (rep_sig 150). *)
+
+(*   Abort. *)
+
 Ltac elim_refinement_types p :=
   (* Step 1 *)
   let f1 := fresh "step_one" in
-  let p2 := eval hnf in p in
-  step_one f1 p2;
+  let p2 := eval hnf in p in (* Maybe we just want p2 to be the body of p, more precisely, we need to check whether p has a body - if it does then we proceed normally, otherwise we still have to figure out what to do *)
+  step_one f1 p2.
 
   (* Step 2 *)
-  let f1 := eval cbn in f1 in
-  let pf_refl := fresh "step_two" in
-  let tp := type of p in
-  let tp := eval red in tp in
-  let tac := ltac2:(f1' p' redPType pf_refl |-
-    let f1'' := Option.get (Ltac1.to_constr f1') in
-    let p'' := Option.get (Ltac1.to_constr p') in
-    let redPType' := Option.get (Ltac1.to_constr redPType) in
-    let eq := make_eq f1'' p'' redPType' in
-    ltac1:(eq' pf_refl' |- assert (pf_refl' : eq') by now simpl) (Ltac1.of_constr eq) pf_refl
-  ) in tac f1 p tp pf_refl.
+  (* let f1 := eval cbn in f1 in *)
+  (* let pf_refl := fresh "step_two" in *)
+  (* let tp := type of p in *)
+  (* let tp := eval red in tp in *)
+  (* let tac := ltac2:(f1' p' redPType pf_refl |- *)
+  (*   let f1'' := Option.get (Ltac1.to_constr f1') in *)
+  (*   let p'' := Option.get (Ltac1.to_constr p') in *)
+  (*   let redPType' := Option.get (Ltac1.to_constr redPType) in *)
+  (*   let eq := make_eq f1'' p'' redPType' in *)
+  (*   ltac1:(eq' pf_refl' |- assert (pf_refl' : eq') by now simpl) (Ltac1.of_constr eq) pf_refl *)
+  (* ) in tac f1 p tp pf_refl. *)
 
   (* (* Step 3 *) *)
   (* let tac := ltac2:(f1' tp' pf_refl' |- *)
@@ -128,17 +174,25 @@ Ltac elim_refinement_types p :=
   (* clear pf_refl. *)
 
 
-Definition P : nat -> Prop := fun x => x >= 3.
+(*   let f1 := eval cbn in step_one in *)
+(*   let pf_refl := fresh "step_two" in *)
+(*   let tp := type of g in *)
+(*   let tp := eval unfold tt in tp in *)
+(*   let tac := ltac2:(f1' p' redPType pf_refl |- *)
+(*     let f1'' := Option.get (Ltac1.to_constr f1') in *)
+(*     let p'' := Option.get (Ltac1.to_constr p') in *)
+(*     let redPType' := Option.get (Ltac1.to_constr redPType) in *)
+(*     let eq := make_eq f1'' p'' redPType' in *)
+(*     ltac1:(eq' |- idtac eq') (Ltac1.of_constr eq) *)
+(*     (* ltac1:(eq' pf_refl' |- assert (pf_refl' : eq') by now simpl) (Ltac1.of_constr eq) pf_refl *) *)
+(*   ) in tac f1 g tp pf_refl. *)
 
-Definition tt := {x : nat | P x}.
 
-Definition v : tt := exist P 3 (le_n 3).
+(*   let f1 := fresh "step_one" in *)
+(*   let p2 := eval hnf in f in *)
+(*   step_one f1 p2. *)
 
-Goal proj1_sig v - 1 >= 2.
-  let f1 := fresh "step_one" in
-  let p2 := eval hnf in v in
-  step_one f1 p2.
-  elim_refinement_types v.
+(*   elim_refinement_types f. *)
 
 Require Import ZArith.
 
@@ -177,11 +231,7 @@ Fixpoint ok' (x : data) : bool :=
         end
   end.
 
-Check @sig.
-
-Definition refData := @sig data (fun r => ok r).
-
-(* Definition refData := { r : data | ok r }. *)
+Definition refData := { r : data | ok r }.
 
 Axiom foo : forall l h , ok (if l <? h then Cons l h Nil else Nil).
 
@@ -191,81 +241,144 @@ Next Obligation.
   exact (foo l h).
 Defined.
 
+
+
+From Ltac2 Require Import Constr Printf Message.
+Ltac2 rec message_of_kind (k : kind) : message :=
+  let sep_msg x y := concat x (concat (of_string ", ") y) in
+  let par_msg msg := concat (of_string "( ") (concat msg (of_string " )")) in
+  match k with
+  | Rel i => of_int i
+  | Var i => concat (of_string "Var ") (of_ident i)
+  | Meta _ => of_string "Meta"
+  | Prod _ b => concat (of_string "Prod ") (message_of_kind (kind b))
+  | Lambda _ b => concat (of_string "Lambda ") (message_of_kind (kind b))
+  | LetIn _ v b =>
+      let msg := sep_msg (message_of_kind (kind v)) (message_of_kind (kind b)) in
+      concat (of_string "LetIn ") (par_msg msg)
+  | App c cs =>
+      let cs_msg_array := Array.map (fun cn => message_of_kind (kind cn)) cs in
+      let cs_msg := Array.fold_left sep_msg (message_of_kind (kind c)) cs_msg_array in
+      concat (of_string "App ") (par_msg cs_msg)
+ (* NOTE: constant is opaque so you can't inspect it (you can't even print it apparently), but you probably can use ltac2 machinery to get a variable whose value corresponds to some coq constant, and then compare it with the constant you have *)
+  | Constant _ _ => of_string "Constant"
+  | Ind _ _ => of_string "Ind"
+  | Constructor _ _ => of_string "Constructor"
+  | Case _ _ _ _ _ => of_string "Case"
+  | _ => of_constr (make k)
+  end.
+
+Ltac2 message_of_constr_opt o :=
+  match o with
+    | None => of_string "None"
+    | Some c => concat (of_string "Some ") (of_constr c)
+  end.
+
+Ltac2 rec print_hyps_list xs :=
+  match xs with
+    | (i, opt, ty) :: tl =>
+        let iM : message := of_string (Ident.to_string i) in
+        let optM : message := message_of_constr_opt opt in
+        let tyM : message := of_constr ty in
+        print (concat iM (concat (of_string " := ") (concat optM (concat (of_string " : ") tyM))));
+        print_hyps_list tl
+    | _ => ()
+  end.
+
+Definition my_identity {A : Type} (x : A) := x.
+
+
+Goal nat -> True.
+  intro y.
+  pose (z := 2).
+  let x := Env.get [Option.get (Ident.of_string "my_identity")] in
+  match x with
+    | Some r => print (of_constr (Env.instantiate r))
+    | _ => print (of_string "boo")
+  end.
+  let a := Control.hyps () in
+  print_hyps_list a.
+
+    let x := constr:(z) in
+    print (message_of_kind (kind x)).
+
+
 Program Definition InBoolRef (x : Z) (s : refData) : bool := InBool x s.
 
 Theorem In_interval: forall x l h, (InBoolRef x (interval l h) = true) <-> l <= x < h.
   Proof.
   split.
   intro H.
+  elim_refinement_types interval.
 
 
-  let f1 := fresh "step_one" in
-  let p2 := eval hnf in InBoolRef in
-  step_one f1 p2.
+(*   let f1 := fresh "step_one" in *)
+(*   let p2 := eval hnf in InBoolRef in *)
+(*   step_one f1 p2. *)
 
-  let f1 := eval cbn in step_one in
-  let tp := type of InBoolRef in idtac tp.
-  let tp := type of InBoolRef in
-  let tp := eval hnf in tp in idtac tp.
+(*   let f1 := eval cbn in step_one in *)
+(*   let tp := type of InBoolRef in idtac tp. *)
+(*   let tp := type of InBoolRef in *)
+(*   let tp := eval hnf in tp in idtac tp. *)
 
-  (* Step 2 *)
-  let f1 := eval cbn in f1 in
-  let pf_refl := fresh "step_two" in
-  let tp := type of p in
-  let tp := eval red in tp in
-  let tac := ltac2:(f1' p' redPType pf_refl |-
-    let f1'' := Option.get (Ltac1.to_constr f1') in
-    let p'' := Option.get (Ltac1.to_constr p') in
-    let redPType' := Option.get (Ltac1.to_constr redPType) in
-    let eq := make_eq f1'' p'' redPType' in
-    ltac1:(eq' pf_refl' |- assert (pf_refl' : eq') by now simpl) (Ltac1.of_constr eq) pf_refl
-  ) in tac f1 p tp pf_refl.
-
-
-
-
+(*   (* Step 2 *) *)
+(*   let f1 := eval cbn in f1 in *)
+(*   let pf_refl := fresh "step_two" in *)
+(*   let tp := type of p in *)
+(*   let tp := eval red in tp in *)
+(*   let tac := ltac2:(f1' p' redPType pf_refl |- *)
+(*     let f1'' := Option.get (Ltac1.to_constr f1') in *)
+(*     let p'' := Option.get (Ltac1.to_constr p') in *)
+(*     let redPType' := Option.get (Ltac1.to_constr redPType) in *)
+(*     let eq := make_eq f1'' p'' redPType' in *)
+(*     ltac1:(eq' pf_refl' |- assert (pf_refl' : eq') by now simpl) (Ltac1.of_constr eq) pf_refl *)
+(*   ) in tac f1 p tp pf_refl. *)
 
 
 
-  (* let f1 := fresh "step_one" in *)
-  (* let p2 := eval hnf in interval in *)
-  (* step_one f1 p2. *)
-
-  (* let tp := type of interval in *)
-  (* let tp := eval red in tp in *)
-  (* let pf_refl := fresh "step_two" in *)
-  (* let tac := ltac2:(f1' p' redPType pf_refl |- *)
-  (*   let f1'' := Option.get (Ltac1.to_constr f1') in *)
-  (*   let p'' := Option.get (Ltac1.to_constr p') in *)
-  (*   let redPType' := Option.get (Ltac1.to_constr redPType) in *)
-  (*   let eq := make_eq f1'' p'' redPType' in *)
-  (*   ltac1:(eq' pf_refl' |- assert (pf_refl' : eq') by now simpl) (Ltac1.of_constr eq) pf_refl *)
-  (* ) in tac step_one interval tp pf_refl. *)
 
 
 
-  (* let tac := ltac2:(f1' tp' pf_refl' |- *)
-  (*     let tp'2 := Option.get (Ltac1.to_constr tp') in *)
-  (*     let (_, pred) := get_ret_sig tp'2 in *)
-  (*     let pred_applied := make_pred (Option.get (Ltac1.to_constr f1')) pred in *)
-  (* (* (*     (* TODO: We really just want to beta reduce one time, maybe head normal form is too strong, maybe a bit of ELPI here would help *) *) *) *)
-  (*     ltac1:(pred' f1'' pf_refl'' |- *)
-  (*       idtac pred') *)
-  (*       (* let pred' := eval cbn in pred' in *) *)
-  (*       (* assert (pred') (*by (rewrite <- pf_refl''; apply proj2_sig)*)) *) (Ltac1.of_constr pred_applied) f1' pf_refl' *)
-  (*   ) *)
-  (* in tac step_one tp step_two. *)
-  (* intros l h. *)
-  (* rewrite (step_two l h). *)
+
+(*   (* let f1 := fresh "step_one" in *) *)
+(*   (* let p2 := eval hnf in interval in *) *)
+(*   (* step_one f1 p2. *) *)
+
+(*   (* let tp := type of interval in *) *)
+(*   (* let tp := eval red in tp in *) *)
+(*   (* let pf_refl := fresh "step_two" in *) *)
+(*   (* let tac := ltac2:(f1' p' redPType pf_refl |- *) *)
+(*   (*   let f1'' := Option.get (Ltac1.to_constr f1') in *) *)
+(*   (*   let p'' := Option.get (Ltac1.to_constr p') in *) *)
+(*   (*   let redPType' := Option.get (Ltac1.to_constr redPType) in *) *)
+(*   (*   let eq := make_eq f1'' p'' redPType' in *) *)
+(*   (*   ltac1:(eq' pf_refl' |- assert (pf_refl' : eq') by now simpl) (Ltac1.of_constr eq) pf_refl *) *)
+(*   (* ) in tac step_one interval tp pf_refl. *) *)
 
 
-  (* elim_refinement_types interval. *)
 
-  (* intros x0 l h. *)
-  (* split. *)
-  (* intro H. *)
-  (* elim_refinement_types fresh_2 interval. *)
-  (* assert (pf_refl : forall l h , fresh_2 l h = proj1_sig (interval l h)) by reflexivity. *)
+(*   (* let tac := ltac2:(f1' tp' pf_refl' |- *) *)
+(*   (*     let tp'2 := Option.get (Ltac1.to_constr tp') in *) *)
+(*   (*     let (_, pred) := get_ret_sig tp'2 in *) *)
+(*   (*     let pred_applied := make_pred (Option.get (Ltac1.to_constr f1')) pred in *) *)
+(*   (* (* (*     (* TODO: We really just want to beta reduce one time, maybe head normal form is too strong, maybe a bit of ELPI here would help *) *) *) *) *)
+(*   (*     ltac1:(pred' f1'' pf_refl'' |- *) *)
+(*   (*       idtac pred') *) *)
+(*   (*       (* let pred' := eval cbn in pred' in *) *) *)
+(*   (*       (* assert (pred') (*by (rewrite <- pf_refl''; apply proj2_sig)*)) *) (Ltac1.of_constr pred_applied) f1' pf_refl' *) *)
+(*   (*   ) *) *)
+(*   (* in tac step_one tp step_two. *) *)
+(*   (* intros l h. *) *)
+(*   (* rewrite (step_two l h). *) *)
 
-  (* elim_refinement_types fresh_1 InBoolRef. *)
-  (* assert (pf_refl : fresh_1 = proj1_sig InBoolRef). *)
+
+(*   (* elim_refinement_types interval. *) *)
+
+(*   (* intros x0 l h. *) *)
+(*   (* split. *) *)
+(*   (* intro H. *) *)
+(*   (* elim_refinement_types fresh_2 interval. *) *)
+(*   (* assert (pf_refl : forall l h , fresh_2 l h = proj1_sig (interval l h)) by reflexivity. *) *)
+
+(*   (* elim_refinement_types fresh_1 InBoolRef. *) *)
+(*   (* assert (pf_refl : fresh_1 = proj1_sig InBoolRef). *) *)
