theories/refinement_elimination_elpi.v
@@ -1,76 +1,193 @@
 From elpi Require Import elpi.
 
+
+(* Elpi Tactic eval_tac. *)
+
+(* Elpi Accumulate lp:{{ *)
+(*   solve (goal _ _ _ _ [trm P] as _G) _GL :- *)
+(*       !, *)
+(*       coq.reduction.lazy.whd P Pr, *)
+(*       coq.say "P: " P, *)
+(*       coq.say "Pr: " Pr. *)
+(* }}. *)
+(* Elpi Typecheck. *)
+
 Elpi Tactic step_one_tac.
 
 Elpi Accumulate lp:{{
   shorten std.{map}.
 
-  pred replace i:term o:term.
-  replace I O :-
-    (copy ({{ exist _ lp:P _ }}) P' :- !, replace P P') =>
-    (copy ({{ @sig lp:A _ }}) A' :- !, replace A A') =>
-    (copy ({{ @proj1_sig _ _ lp:X }}) X' :- !, replace X X') =>
-      copy I O.
 
-
-%  pred replace i:term, o:term.
+  % Maybe this thing is working, but the evaluation did not expand the symbol inside the lambda
 %  replace I O :-
-%            (copy ({{ exist _ lp:P _ }}) P' :- !, replace P P') =>
-%            (copy ({{ @sig lp:A _ }}) A' :- !, replace A A') =>
-%            (copy ({{ @proj1_sig _ _ lp:X }}) X' :- !, replace X X') =>
-%              copy I O.
+%    (copy {{ 2%nat }} {{ 3%nat }}) => copy I O.
+%    (copy ({{ exist _ lp:P _ }}) P) =>
+%    (copy ({{ @sig lp:A _ }}) A) =>
+%    (copy ({{ @proj1_sig _ _ lp:X }}) X) =>
+%          copy I O.
 
-%  replace T T' :-
-%            coq.unify-leq T ({{ exist _ lp:P _ }}) ok, !, replace P T'.
-%  replace T T' :-
-%            coq.unify-leq T ({{ @sig lp:A _ }}) ok, !, replace A T'.
-%  replace T T' :-
-%            coq.unify-leq T ({{ @proj1_sig _ _ lp:X }}) ok, !, replace X T'.
+
+  pred refinefull i:term.
+  pred refinefull_rec i:term.
+
+  refinefull_rec ({{ exist _ _ _ }}) :- !.
+  refinefull_rec ({{ @sig _ _ }}) :- !.
+  refinefull_rec ({{ @proj1_sig _ _ _ }}) :- !.
+
+  refinefull_rec (fun _ T _) :-
+    refinefull T, !.
+  refinefull_rec (fun _ T F) :-
+    pi x\ decl x _ T => refinefull (F x), !.
+
+  refinefull_rec (let _ T _ _) :-
+    refinefull T, !.
+  refinefull_rec (let _ _ B _) :-
+    refinefull B, !.
+  refinefull_rec (let _ T _ F) :-
+    pi x\ decl x _ T => refinefull (F x), !.
+
+  refinefull_rec (prod _ T _) :-
+    refinefull T, !.
+  refinefull_rec (prod _ T F) :-
+    pi x\ decl x _ T => refinefull (F x), !.
+
+  refinefull_rec (app L) :- !, std.exists L refinefull.
+
+  refinefull_rec (fix _ _ Ty _) :-
+    refinefull Ty, !.
+  refinefull_rec (fix _ _ Ty F) :-
+    pi x\ decl x _ Ty => refinefull (F x), !.
+
+  refinefull_rec (match T _ _) :-
+    refinefull T, !. %, coq.say "match 1".
+  refinefull_rec (match _ Rty _) :-
+    refinefull Rty, !. %, coq.say "match 2".
+  refinefull_rec (match _ _ B) :-
+    std.exists B refinefull, !. %, coq.say "match 3".
+
+  refinefull_rec (uvar _ L) :- std.exists L refinefull, !.
+
+  refinefull I :-
+    coq.reduction.lazy.whd I Ir,
+    %coq.say "refinefull exist 2",
+    refinefull_rec Ir.
+
+
+
+
+
+  pred smart_refineexp i:term o:term.
+  pred refineexp i:term o:term.
+  pred refineexp_rec i:term o:term.
+
+  smart_refineexp I O :-
+    refinefull I, !, refineexp I O.
+  smart_refineexp I I.
+
+  refineexp I O :-
+    coq.reduction.lazy.whd I Ir,
+    smart_refineexp Ir O.
+
+  refineexp_rec (fun X T F) (fun X T' F') :- !,
+    smart_refineexp T T',
+    pi x\ decl x _ T => pi x'\ decl x' _ T' => smart_refineexp (F x) (F' x').
+
+  refineexp_rec I I.
+
+
+
+  pred smart_replace i:term o:term.
+  pred red_replace i:term o:term.
+  pred replace i:term o:term.
+
+  smart_replace I O :-
+    %coq.say "smart_replace 0",
+    refinefull I, !,
+    %coq.say "smart_replace 1",
+    %coq.term->string I Is,
+    %coq.say "I = " Is,
+    red_replace I O.
+    %coq.term->string O Os.
+    %coq.say "O = " Os.
+
+
+  smart_replace I I.% :-
+    %coq.say "smart_replace 2",
+    %coq.term->string I Is,
+    %coq.say "I = " Is.
+
+  red_replace I O :-
+    coq.say "red_replace",
+    coq.reduction.lazy.whd I Ir,
+    %coq.term->string I Is,
+    %coq.say "I = " Is,
+    %coq.term->string Ir Irs,
+    %coq.say "Ir = " Irs,
+    replace Ir O.
+    %coq.term->string I Is,
+    %coq.term->string Ir Irs,
+    %coq.term->string O Os,
+    %coq.say "I = " Is,
+    %coq.say "Irs = " Irs,
+    %coq.say "O = " Os.
+
+
+%  replace ({{ exist _ lp:P _ }}) T' :- !, coq.say "replace exist", smart_replace P T'.
+%  replace ({{ @proj1_sig _ _ lp:X }}) T' :- !, smart_replace X T'.
+%  replace ({{ @sig lp:A _ }}) T' :- ! , smart_replace A T'.
 %  replace X Y :- name X, !, X = Y, !. % avoid loading "replace x x" at binders
 %  replace (global _ as C) C :- !.
 %  replace (pglobal _ _ as C) C :- !.
 %  replace (sort _ as C) C :- !.
 %  replace (fun N T F) (fun N T1 F1) :- !,
-%    replace T T1, pi x\ decl x _ T => pi x1\ decl x1 _ T1 => replace x x1 => replace (F x) (F1 x1).
+%    smart_replace T T1, pi x\ decl x _ T => pi x1\ decl x1 _ T1 => smart_replace x x1 => smart_replace (F x) (F1 x1).
 %  replace (let N T B F) (let N T1 B1 F1) :- !,
-%    replace T T1, replace B B1, pi x\ decl x _ T => pi x1\ decl x1 _ T1 => replace x x1 => replace (F x) (F1 x1).
+%    smart_replace T T1, smart_replace B B1, pi x\ decl x _ T => pi x1\ decl x1 _ T1 => smart_replace x x1 => smart_replace (F x) (F1 x1).
 %  replace (prod N T F) (prod N T1 F1) :- !,
-%    replace T T1, (pi x\ decl x _ T => pi x1\ decl x1 _ T1 => replace x x1 => replace (F x) (F1 x1)).
-%  replace (app L) (app L1) :- !, map L replace L1.
+%    smart_replace T T1, (pi x\ decl x _ T => pi x1\ decl x1 _ T1 => smart_replace x x1 => smart_replace (F x) (F1 x1)).
+%  replace (app L) (app L1) :- !,
+%    map L smart_replace L1.
 %  replace (fix N Rno Ty F) (fix N Rno Ty1 F1) :- !,
-%    replace Ty Ty1, pi x\ decl x _ Ty => pi x1\ decl x1 _ Ty1 => replace x x1 => replace (F x) (F1 x1).
+%    smart_replace Ty Ty1, pi x\ decl x _ Ty => pi x1\ decl x1 _ Ty1 => smart_replace x x1 => smart_replace (F x) (F1 x1).
 %  replace (match T Rty B) (match T1 Rty1 B1) :- !,
-%    replace T T1, replace Rty Rty1, map B replace B1.
+%    smart_replace T T1, smart_replace Rty Rty1, map B smart_replace B1.
 %  replace (primitive _ as C) C :- !.
-%  replace (uvar M L as X) W :- var X, !, map L replace L1, coq.mk-app-uvar M L1 W.
+%  replace (uvar M L as X) W :- var X, !, map L smart_replace L1, coq.mk-app-uvar M L1 W.
 %  % when used in CHR rules
-%  replace (uvar X L) (uvar X L1) :- map L replace L1.
+%  replace (uvar X L) (uvar X L1) :- map L smart_replace L1.
 
-
-%  pred step_one'' i:term, o:term.
-%  step_one'' I O :-
-%      coq.say "step_one'' before: I = " I " | O = " O,
-%      (copy ( {{ exist _ lp:P _ }} ) P :- !) => copy I O,
-%      coq.say "step_one'' after: I = " I " | O = " O.
-%
-%  pred step_one' i:term o:term.
-%  step_one' I O :-
-%      coq.say "step_one' before: I = " I " | O = " O,
-%      (step_one'' ( {{ @sig lp:A _  }} ) A :- !) => step_one'' I O,
-%      coq.say "step_one' after: I = " I " | O = " O.
-%
-%  pred step_one i:term o:term.
-%  step_one I O :-
-%      coq.say "step_one before: I = " I " | O = " O,
-%      (step_one' ( {{ proj1_sig lp:X }} ) X :- !) => step_one' I O,
-%      coq.say "step_one after: I = " I " | O = " O.
+  pred replace i:term, o:term.
+  replace ({{ exist _ lp:P _ }}) P' :- !, replace P P'.
+  replace ({{ @sig lp:A _ }}) A' :- !, replace A A'.
+  replace ({{ @proj1_sig _ _ lp:X }}) X' :- !, replace X X'.
+  replace X Y :- name X, !, X = Y, !. % avoid loading "replace x x" at binders
+  replace (global _ as C) C :- !.
+  replace (pglobal _ _ as C) C :- !.
+  replace (sort _ as C) C :- !.
+  replace (fun N T F) (fun N T1 F1) :- !,
+    replace T T1, pi x\ decl x _ T => pi x1\ decl x1 _ T1 => replace x x1 => replace (F x) (F1 x1).
+  replace (let N T B F) (let N T1 B1 F1) :- !,
+    replace T T1, replace B B1, pi x\ decl x _ T => pi x1\ decl x1 _ T1 => replace x x1 => replace (F x) (F1 x1).
+  replace (prod N T F) (prod N T1 F1) :- !,
+    replace T T1, (pi x\ decl x _ T => pi x1\ decl x1 _ T1 => replace x x1 => replace (F x) (F1 x1)).
+  replace (app L) (app L1) :- !, map L replace L1.
+  replace (fix N Rno Ty F) (fix N Rno Ty1 F1) :- !,
+    replace Ty Ty1, pi x\ decl x _ Ty => pi x1\ decl x1 _ Ty1 => replace x x1 => replace (F x) (F1 x1).
+  replace (match T Rty B) (match T1 Rty1 B1) :- !,
+    replace T T1, replace Rty Rty1, map B replace B1.
+  replace (primitive _ as C) C :- !.
+  replace (uvar M L as X) W :- var X, !, map L replace L1, coq.mk-app-uvar M L1 W.
+  % when used in CHR rules
+  replace (uvar X L) (uvar X L1) :- map L replace L1.
 
   solve (goal _ _ _ _ [str S, trm P] as G) GL :-
       !,
       coq.string->name S N,
       replace P P',
-      coq.say "input of replace: " P,
-      coq.say "replace computed: " P',
+      coq.term->string P Ps,
+      coq.term->string P' P's,
+      coq.say "P: " Ps,
+      coq.say "Pr': " P's,
 
       refine (let N _ P' Tgt_) G GL.
 
