theories/sig_expand_elpi.v
@@ -1,0 +1,116 @@
+From elpi Require Import elpi.
+
+
+Elpi Tactic sig_expand_tac.
+
+Elpi Accumulate lp:{{
+
+  pred sigfull i:term.
+  pred sigfull_rec i:term.
+
+  sigfull_rec ({{ @sig _ _ }}).
+
+  sigfull_rec (fun _ T _) :-
+    sigfull T.
+  sigfull_rec (fun _ T F) :-
+    pi x\ decl x _ T => sigfull (F x).
+
+  sigfull_rec (let _ T _ _) :-
+    sigfull T.
+  sigfull_rec (let _ _ B _) :-
+    sigfull B.
+  sigfull_rec (let _ T _ F) :-
+    pi x\ decl x _ T => sigfull (F x).
+
+  sigfull_rec (prod _ T _) :-
+    sigfull T.
+  sigfull_rec (prod _ T F) :-
+    pi x\ decl x _ T => sigfull (F x).
+
+  sigfull_rec (app L) :- std.exists L sigfull.
+
+  sigfull_rec (fix _ _ Ty _) :-
+    sigfull Ty.
+  sigfull_rec (fix _ _ Ty F) :-
+    pi x\ decl x _ Ty => sigfull (F x).
+
+  sigfull_rec (match T _ _) :-
+    sigfull T.
+  sigfull_rec (match _ Rty _) :-
+    sigfull Rty.
+  sigfull_rec (match _ _ B) :-
+    std.exists B sigfull.
+
+  sigfull_rec (uvar _ L) :- std.exists L sigfull.
+
+  sigfull I :-
+    coq.reduction.lazy.whd I Ir,
+    sigfull_rec Ir.
+
+  pred smart_sig_expand i:term o:term.
+  pred sig_expand i:term o:term.
+  pred sig_expand_rec i:term o:term.
+
+  smart_sig_expand I O :-
+    sigfull I, !,
+    coq.term->string I Is,
+    coq.say "smart_sig_expand sigfull: Is = " Is,
+    sig_expand I O,
+    coq.term->string O Os,
+    coq.say "smart_sig_expand sigfull: Os = " Os.
+  smart_sig_expand I I :-
+    coq.term->string I Is,
+    coq.say "smart_sig_expand sigless: Is = " Is.
+
+  sig_expand I O :-
+    coq.reduction.lazy.whd I Ir,
+    sig_expand_rec Ir O.
+
+% There probably is a more direct algorithm that simultaneously checks whether there is a `sig` inside the term and
+% expands. Chantal's idea: as we traverse the tree, remember which constructors we went through and rebuild then when
+% we find a `sig`.
+% Another approach would be to understand how to use memoization
+  %sig_expand_rec X Y :- name X, !, X = Y, !. % avoid loading "replace x x" at binders
+  sig_expand_rec (global _ as C) C :- coq.say "global", !.
+  sig_expand_rec (pglobal _ _ as C) C :- coq.say "pglobal", !.
+  sig_expand_rec (sort _ as C) C :- coq.say "sort", !.
+  sig_expand_rec (fun N T F) (fun N T1 F1) :- coq.say "fun", !,
+    smart_sig_expand T T1, pi x\ decl x _ T => smart_sig_expand (F x) (F1 x).
+  sig_expand_rec (let N T B F) (let N T1 B1 F1) :- coq.say "let", !,
+    smart_sig_expand T T1, smart_sig_expand B B1, pi x\ decl x _ T => smart_sig_expand (F x) (F1 x).
+  sig_expand_rec (prod N T F) (prod N T1 F1) :- coq.say "prod", !,
+    smart_sig_expand T T1, (pi x\ decl x _ T => smart_sig_expand (F x) (F1 x)).
+  sig_expand_rec (app L as T) (app L1) :-
+    coq.term->string T Ts,
+    coq.say "app: " Ts, !,
+    %(F X1 X2 :- smart_sig_expand B X1 X2) =>
+    std.map L smart_sig_expand L1.
+  sig_expand_rec (fix N Rno Ty F) (fix N Rno Ty1 F1) :- coq.say "fix", !,
+    smart_sig_expand Ty Ty1, pi x\ decl x _ Ty => smart_sig_expand (F x) (F1 x).
+  sig_expand_rec (match T Rty B) (match T1 Rty1 B1) :- coq.say "match", !,
+    smart_sig_expand T T1, smart_sig_expand Rty Rty1,
+    %(F X1 X2 :- smart_sig_expand BB X1 X2) =>
+    std.map B smart_sig_expand B1.
+  sig_expand_rec (primitive _ as C) C :- coq.say "primitive", !.
+  sig_expand_rec (uvar M L as X) W :- coq.say "uvar", var X, !,
+    %(F X1 X2 :- smart_sig_expand B X1 X2) =>
+   std.map L smart_sig_expand L1, coq.mk-app-uvar M L1 W.
+  % when used in CHR rules
+  sig_expand_rec (uvar X L) (uvar X L1) :- coq.say "uvar2",
+    %(F X1 X2 :- smart_sig_expand B X1 X2) =>
+      std.map L smart_sig_expand L1.
+
+  solve (goal _ _ _ _ [str S, trm P] as G) GL :-
+      !,
+      coq.string->name S N,
+      smart_sig_expand P P',
+      refine (let N _ P' Tgt_) G GL.
+
+  solve (goal _ _ _ _ [_, trm _]) _ :- coq.ltac.fail 0 "The first argument should be an identifier".
+
+  solve (goal _ _ _ _ [_, _]) _ :- coq.ltac.fail 0 "The second argument should be a term".
+
+  solve (goal _ _ _ _ _) _ :- coq.ltac.fail 0 "There should be exactly two arguments".
+
+}}.
+Elpi Typecheck.
